Source/DafnyCompilers/Printer.dfy
@@ -1,0 +1,23 @@
+include "Semantics.dfy"
+include "Library.dfy"
+include "CSharpDafnyInterop.dfy"
+
+module Interp.Printer {
+  import Values
+  import opened Lib
+  import Interop = CSharpDafnyInterop
+
+  function method ToString(v: Values.T) : string {
+    match v
+      case Bool(b) => Str.of_bool(b)
+      case Char(c) => Str.of_char(c)
+      case Int(i) => Str.of_int(i)
+      case Real(r) => var (n, d) := Interop.Reals.AsIntegerRatio(r); Str.of_int(n) + "/" + Str.of_int(d)
+      case BigOrdinal(o) => "<*>" // FIXME
+      case BitVector(value) => "bv(" + Str.of_int(value, 16) + ")"
+      case Map(m) => "map[" + "<*>" + "]" // FIXME iterate over map
+      case Multiset(ms) => "multiset{" + "<*>" + "}]" // FIXME iterate over multiset (convert to map?)
+      case Seq(sq) => "[" + Lib.Str.Join(",", Lib.Seq.Map(v requires v in sq => ToString(v), sq)) + "]"
+      case Set(st) => "set{" + "<*>" + "}" // FIXME iterate over set
+  }
+}
