Source/DafnyCompilers/REPL/Repl.dfy
@@ -1,0 +1,42 @@
+include "../Semantics.dfy"
+include "../CompilerCommon.dfy"
+include "../Printer.dfy"
+include "../Library.dfy"
+include "../CSharpDafnyASTModel.dfy"
+
+import C = CSharpDafnyASTModel
+import D = DafnyCompilerCommon
+import opened Lib.Datatypes
+
+type Expr = D.AST.Expr.Expr
+
+method {:extern "Read"} Read() returns (e: C.Expression)
+
+function method Translate(cE: C.Expression) : (o: Option<Expr>)
+  ensures o.Some? ==> Interp.SupportsInterp(o.t)
+  reads *
+{
+  var e := D.Translator.TranslateExpression(cE);
+  if Interp.SupportsInterp(e) then Some(e) else None
+}
+
+function method Eval(e: Expr) : Values.T
+  requires Interp.SupportsInterp(e)
+{
+  Interp.InterpExpr(e).1
+}
+
+method Main()
+  decreases *
+{
+  while true
+    decreases *
+  {
+    var cExpr := Read();
+    match Translate(cExpr)
+      case None => print "Unsupported expression";
+      case Some(e) =>
+        var val := Eval(e);
+        print Interp.Printer.ToString(val);
+  }
+}
